attempt to prove TRANS_correct, but going backwards
trying to work out a good definition of sequent, and the interplay with
has_meaning led me to realise that the syntactic inference system
probably needs to be different: it needs to be restricted to terms with
semantics only, but this has to be done by syntactic checks only
(probably by keeping track of what terms the kernel has produced).

indeed, the theorem REFL_correct proved before is useless for soundness,
since it assumes the term has_meaning, which the syntactic kernel won't
(and can't directly) check for.

hol-light/sholSemanticsScript.sml
@@ -194,27 +194,8 @@ val term_valuation_def = Define`
   term_valuation τ σ ⇔
     FEVERY (λ(v,m). ∃mty. typeset τ (SND v) mty ∧ m <: mty) σ`
 
-val _ = Parse.add_infix("|=",450,Parse.NONASSOC)
-
 val _ = Parse.add_infix("closes_over",450,Parse.NONASSOC)
 val _ = Parse.overload_on("closes_over",``λσ t. ∀x ty. VFREE_IN (Var x ty) t ⇒ (x,ty) ∈ FDOM σ``)
-
-val has_meaning_def = Define`
-  has_meaning t =
-           ∀σ τ. type_valuation τ ∧
-                 term_valuation τ σ ∧
-                 σ closes_over t
-                 ⇒
-                 ∃m. semantics σ τ t m`
-
-val sequent_def = xDefine"sequent"`
-  h |= c ⇔ EVERY (λt. t has_type Bool) (c::h) ∧
-           ∀σ τ. type_valuation τ ∧
-                 term_valuation τ σ ∧
-                 EVERY (λt. semantics σ τ t true) h ∧
-                 (∀x ty. VFREE_IN (Var x ty) c ⇒ (x,ty) ∈ FDOM σ)
-                 ⇒
-                 semantics σ τ c true`
 
 val typeset_inhabited = store_thm("typeset_inhabited",
   ``∀ty τ mty. type_valuation τ ∧ typeset τ ty mty ⇒ ∃m. m <: mty``,
@@ -419,35 +400,6 @@ val semantics_closes_over = store_thm("semantics_closes_over",
     fs[FDOM_FUPDATE] >>
     metis_tac[]))
 
-val semantics_equation = store_thm("semantics_equation",
-  ``∀σ τ s t mty ms mt.
-    type_valuation τ ∧ term_valuation τ σ ∧
-    semantics σ τ s ms ∧ semantics σ τ t mt ∧
-    (typeof s = typeof t)
-    ⇒ semantics σ τ (s === t) (boolean (ms = mt))``,
-  rw[equation_def] >>
-  simp[Once semantics_cases] >>
-  simp[Once semantics_cases] >>
-  simp[Once semantics_cases] >>
-  srw_tac[DNF_ss][] >>
-  imp_res_tac semantics_typeset >> simp[] >>
-  map_every qexists_tac[`mt`,`ms`,`mty`] >> simp[] >>
-  match_mp_tac EQ_SYM >>
-  qho_match_abbrev_tac`apply (apply (abstract a b f) x) y = z` >>
-  `apply (abstract a b f) x = f x` by (
-    match_mp_tac APPLY_ABSTRACT >>
-    unabbrev_all_tac >> simp[] >>
-    conj_tac >- metis_tac[semantics_typeset,semantics_11,WELLTYPED] >>
-    match_mp_tac ABSTRACT_IN_FUNSPACE >>
-    metis_tac[semantics_typeset,WELLTYPED,BOOLEAN_IN_BOOLSET] ) >>
-  simp[Abbr`f`,Abbr`b`] >>
-  qho_match_abbrev_tac`apply (abstract a b f) y = z` >>
-  `apply (abstract a b f) y = f y `  by (
-    match_mp_tac APPLY_ABSTRACT >>
-    unabbrev_all_tac >> simp[] >>
-    metis_tac[semantics_typeset,semantics_11,WELLTYPED,BOOLEAN_IN_BOOLSET] ) >>
-  unabbrev_all_tac >> simp[])
-
 val semantics_raconv = store_thm("semantics_raconv",
   ``∀env tp.
       RACONV env tp ⇒
@@ -541,21 +493,6 @@ val semantics_aconv = store_thm("semantics_aconv",
   rw[] >> first_x_assum match_mp_tac >> rw[] >>
   fs[ALPHAVARS_def])
 
-val binary_inference_rule = store_thm("binary_inference_rule",
-  ``p1 has_type Bool ∧ p2 has_type Bool ∧ q has_type Bool ∧
-    (∀σ τ. type_valuation τ ∧ term_valuation τ σ ∧
-           (σ closes_over p1 ⇒ semantics σ τ p1 true) ∧
-           (σ closes_over p2 ⇒ semantics σ τ p2 true) ∧
-           σ closes_over q
-         ⇒ semantics σ τ q true)
-    ⇒ h1 |= p1 ∧ h2 |= p2 ⇒ TERM_UNION h1 h2 |= q``,
-  rw[sequent_def,ALL_BOOL_TERM_UNION] >>
-  first_x_assum match_mp_tac >> simp[] >>
-  conj_tac >> strip_tac >>
-  first_x_assum match_mp_tac >> rw[] >>
-  fs[EVERY_MEM] >> rw[] >>
-  metis_tac[TERM_UNION_THM,semantics_aconv,welltyped_def,TERM_UNION_NONEW])
-
 val semantics_vfree_in = store_thm("semantics_vfree_in",
   ``∀τ σ1 σ2 t.
       type_valuation τ ∧
@@ -592,14 +529,119 @@ val semantics_vfree_in = store_thm("semantics_vfree_in",
     fs[] >> metis_tac[] ) >>
   fs[] )
 
+val type_valuation_exists = store_thm("type_valuation_exists",
+  ``∃τ. type_valuation τ``,
+  rw[type_valuation_def,GSYM SKOLEM_THM] >>
+  metis_tac[BOOLEAN_IN_BOOLSET])
+
+val has_meaning_def = Define`
+  has_meaning t = ∀τ σ. type_valuation τ ∧ term_valuation τ σ ⇒
+    ∃σ' m. σ ⊑ σ' ∧ term_valuation τ σ' ∧ σ' closes_over t ∧
+           semantics σ' τ t m`
+
+val has_meaning_welltyped = store_thm("has_meaning_welltyped",
+  ``has_meaning t ⇒ welltyped t``,
+  rw[has_meaning_def] >>
+  metis_tac[type_valuation_exists,semantics_typeset
+           ,term_valuation_def,CONJUNCT1 FEVERY_STRENGTHEN_THM
+           ,SUBMAP_FEMPTY])
+
+val closes_over_aconv = store_thm("closes_over_aconv",
+  ``∀σ t t'. σ closes_over t ∧ ACONV t t' ⇒ σ closes_over t'``,
+  rw[] >> metis_tac[VFREE_IN_ACONV])
+
+val RACONV_welltyped = store_thm("RACONV_welltyped",
+  ``∀t1 env t2.
+    EVERY (λ(x,y). welltyped x ∧ welltyped y ∧ typeof x = typeof y) env ∧
+    welltyped t1 ∧ RACONV env (t1,t2) ⇒
+    welltyped t2``,
+  Induct >>
+  simp[Once RACONV_cases] >- (
+    rw[] >> rw[WELLTYPED_CLAUSES] )
+  >- (
+    rw[WELLTYPED_CLAUSES] >>
+    pop_assum mp_tac >>
+    simp[Once RACONV_cases] >>
+    rw[] >> rw[WELLTYPED_CLAUSES] >>
+    metis_tac[RACONV_TYPE,FST,SND] )
+  >- (
+    rw[Once RACONV_cases] >>
+    pop_assum mp_tac >>
+    rw[Once RACONV_cases] >>
+    rw[WELLTYPED_CLAUSES] >>
+    first_x_assum match_mp_tac >>
+    qmatch_assum_abbrev_tac`RACONV env' pp` >>
+    qexists_tac`env'` >>
+    simp[Abbr`env'`]))
+
+val ACONV_welltyped = store_thm("ACONV_welltyped",
+  ``∀t1 t2. ACONV t1 t2 ∧ welltyped t1 ⇒ welltyped t2``,
+  rw[ACONV_def] >>
+  metis_tac[RACONV_welltyped,EVERY_DEF])
+
+val has_meaning_aconv = store_thm("has_meaning_aconv",
+  ``has_meaning t ∧ ACONV t t' ⇒ has_meaning t'``,
+  rw[] >>
+  imp_res_tac has_meaning_welltyped >>
+  fs[has_meaning_def] >> rw[] >>
+  metis_tac[semantics_aconv,closes_over_aconv,ACONV_welltyped])
+
+val semantics_equation = store_thm("semantics_equation",
+  ``∀σ τ s t mty ms mt mst.
+    type_valuation τ ∧ term_valuation τ σ ∧
+    semantics σ τ s ms ∧ semantics σ τ t mt ∧
+    (typeof s = typeof t) ∧ mst = boolean (ms = mt)
+    ⇒ semantics σ τ (s === t) mst``,
+  rw[equation_def] >>
+  simp[Once semantics_cases] >>
+  simp[Once semantics_cases] >>
+  simp[Once semantics_cases] >>
+  srw_tac[DNF_ss][] >>
+  imp_res_tac semantics_typeset >> simp[] >>
+  map_every qexists_tac[`mt`,`ms`,`mty`] >> simp[] >>
+  match_mp_tac EQ_SYM >>
+  qho_match_abbrev_tac`apply (apply (abstract a b f) x) y = z` >>
+  `apply (abstract a b f) x = f x` by (
+    match_mp_tac APPLY_ABSTRACT >>
+    unabbrev_all_tac >> simp[] >>
+    conj_tac >- metis_tac[semantics_typeset,semantics_11,WELLTYPED] >>
+    match_mp_tac ABSTRACT_IN_FUNSPACE >>
+    metis_tac[semantics_typeset,WELLTYPED,BOOLEAN_IN_BOOLSET] ) >>
+  simp[Abbr`f`,Abbr`b`] >>
+  qho_match_abbrev_tac`apply (abstract a b f) y = z` >>
+  `apply (abstract a b f) y = f y `  by (
+    match_mp_tac APPLY_ABSTRACT >>
+    unabbrev_all_tac >> simp[] >>
+    metis_tac[semantics_typeset,semantics_11,WELLTYPED,BOOLEAN_IN_BOOLSET] ) >>
+  unabbrev_all_tac >> simp[])
+
+val _ = Parse.add_infix("|=",450,Parse.NONASSOC)
+
+val sequent_def = xDefine"sequent"`
+  h |= c ⇔ EVERY (λt. t has_type Bool) (c::h) ∧
+           EVERY has_meaning (c::h) ∧
+           ∀σ τ. type_valuation τ ∧
+                 term_valuation τ σ ∧
+                 EVERY (λt. semantics σ τ t true) h ∧
+                 σ closes_over c
+                 ⇒
+                 semantics σ τ c true`
+
 val vfree_in_equation = store_thm("vfree_in_equation",
   ``VFREE_IN v (s === t) ⇔ (v = Equal (typeof s)) ∨ VFREE_IN v s ∨ VFREE_IN v t``,
   rw[equation_def,VFREE_IN_def] >> metis_tac[])
 
+val closes_over_equation = store_thm("closes_over_equation",
+  ``σ closes_over l === r ⇔ σ closes_over l ∧ σ closes_over r``,
+  rw[vfree_in_equation] >> metis_tac[])
+
+(*
 val ASSUME_correct = store_thm("ASSUME_correct",
   ``∀p. p has_type Bool ⇒ [p] |= p``,
   rw[sequent_def])
+*)
 
+(*
 val REFL_correct = store_thm("REFL_correct",
   ``∀t. has_meaning t ∧ welltyped t ⇒ [] |= t === t``,
   rw[sequent_def,WELLTYPED,EQUATION_HAS_TYPE_BOOL] >>
@@ -610,6 +652,58 @@ val REFL_correct = store_thm("REFL_correct",
   `true = boolean (mt = mt)` by rw[boolean_def] >> pop_assum SUBST1_TAC >>
   match_mp_tac semantics_equation >>
   metis_tac[WELLTYPED,semantics_typeset])
+*)
+
+(*
+val binary_inference_rule = store_thm("binary_inference_rule",
+  ``∀h1 h2 p1 p2 q.
+    (p1 has_type Bool ∧ p2 has_type Bool ⇒ q has_type Bool) ∧
+    (has_meaning p1 ∧ has_meaning p2 ⇒ has_meaning q) ∧
+    (∀σ τ. type_valuation τ ∧ term_valuation τ σ ∧
+           semantics σ τ p1 true ∧ semantics σ τ p2 true ∧
+           σ closes_over q ⇒
+           semantics σ τ q true) ∧
+    h1 |= p1 ∧ h2 |= p2
+    ⇒ TERM_UNION h1 h2 |= q``,
+  rpt gen_tac >> strip_tac >>
+  fs[sequent_def,ALL_BOOL_TERM_UNION] >>
+  conj_tac >- (
+    fs[EVERY_MEM] >>
+    metis_tac[TERM_UNION_NONEW,TERM_UNION_THM,has_meaning_aconv] ) >>
+  rw[] >>
+
+  simp[sequent_def,ALL_BOOL_TERM_UNION] >>
+  first_x_assum match_mp_tac >> simp[] >>
+  conj_tac >> strip_tac >>
+  first_x_assum match_mp_tac >> simp[] >>
+  fs[EVERY_MEM] >>
+  metis_tac[TERM_UNION_THM,semantics_aconv,welltyped_def
+           ,TERM_UNION_NONEW,semantics_closes_over])
+*)
+
+(*
+val TRANS_correct = store_thm("TRANS_correct",
+  ``∀h1 h2 l m1 m2 r.
+      h1 |= l === m1 ∧ h2 |= m2 === r ∧ ACONV m1 m2
+      ⇒ TERM_UNION h1 h2 |= l === r``,
+  rw[] >> match_mp_tac binary_inference_rule >>
+  map_every qexists_tac[`l === m1`,`m2 === r`] >>
+  simp[EQUATION_HAS_TYPE_BOOL] >>
+  conj_tac >- metis_tac[ACONV_TYPE] >>
+  rw[] >> match_mp_tac semantics_equation >>
+  sequent_def
+  simp[boolean_def] >>
+  fs[closes_over_equation] >>
+  semantics_closes_over
+  sequent_def
+
+  semantics_equation
+  semantics_aconv
+  closes_over
+  semantics_closes_over
+  print_find"aconv_boolean"
+  sequent_def
+*)
 
 val _ = export_theory()
 
